src/Lean/Server/FileWorker/RequestHandling.lean
@@ -251,8 +251,9 @@ partial def handleDocumentSymbol (_ : DocumentSymbolParams)
     stxs := stxs ++ (← parseAhead doc.meta.mkInputContext lastSnap).toList
     let (syms, _) := toDocumentSymbols doc.meta.text stxs
     return { syms := syms.toArray }
-  where
-    toDocumentSymbols (text : FileMap)
+where
+  toDocumentSymbols (text : FileMap) (stxs : List Syntax) : List DocumentSymbol × List Syntax :=
+    match stxs with
     | [] => ([], [])
     | stx::stxs => match stx with
       | `(namespace $id)  => sectionLikeToDocumentSymbols text stx stxs (id.getId.toString) SymbolKind.namespace id
@@ -263,12 +264,15 @@ partial def handleDocumentSymbol (_ : DocumentSymbolParams)
         unless stx.isOfKind ``Lean.Parser.Command.declaration do
           return (syms, stxs')
         if let some stxRange := stx.getRange? then
-          let (name, selection) := match stx with
+          let (name, selection) : String × Syntax := match stx with
             | `($_:declModifiers $_:attrKind instance $[$np:namedPrio]? $[$id:ident$[.{$ls,*}]?]? $sig:declSig $_) =>
               ((·.getId.toString) <$> id |>.getD s!"instance {sig.raw.reprint.getD ""}", id.map (·.raw) |>.getD sig)
-            | _ => match stx[1][1] with
-              | `(declId|$id:ident$[.{$ls,*}]?) => (id.getId.toString, id)
-              | _                               => (stx[1][0].isIdOrAtom?.getD "<unknown>", stx[1][0])
+            | _ =>
+              match stx.getArg 1 |>.getArg 1 with
+              | `(declId|$id:ident$[.{$ls,*}]?) => (id.raw.getId.toString, id)
+              | _ =>
+                let stx10 : Syntax := (stx.getArg 1).getArg 0 -- TODO: stx[1][0] times out
+                (stx10.isIdOrAtom?.getD "<unknown>", stx10)
           if let some selRange := selection.getRange? then
             return (DocumentSymbol.mk {
               name := name
@@ -277,22 +281,23 @@ partial def handleDocumentSymbol (_ : DocumentSymbolParams)
               selectionRange := selRange.toLspRange text
               } :: syms, stxs')
         return (syms, stxs')
-    sectionLikeToDocumentSymbols (text : FileMap) (stx : Syntax) (stxs : List Syntax) (name : String) (kind : SymbolKind) (selection : Syntax) :=
-        let (syms, stxs') := toDocumentSymbols text stxs
-        -- discard `end`
-        let (syms', stxs'') := toDocumentSymbols text (stxs'.drop 1)
-        let endStx := match stxs' with
-          | endStx::_ => endStx
-          | []        => (stx::stxs').getLast!
-        -- we can assume that commands always have at least one position (see `parseCommand`)
-        let range := (mkNullNode #[stx, endStx]).getRange?.get!.toLspRange text
-        (DocumentSymbol.mk {
-          name
-          kind
-          range
-          selectionRange := selection.getRange? |>.map (·.toLspRange text) |>.getD range
-          children? := syms.toArray
-        } :: syms', stxs'')
+
+  sectionLikeToDocumentSymbols (text : FileMap) (stx : Syntax) (stxs : List Syntax) (name : String) (kind : SymbolKind) (selection : Syntax) : List DocumentSymbol × List Syntax :=
+    let (syms, stxs') := toDocumentSymbols text stxs
+    -- discard `end`
+    let (syms', stxs'') := toDocumentSymbols text (stxs'.drop 1)
+    let endStx := match stxs' with
+      | endStx::_ => endStx
+      | []        => (stx::stxs').getLast!
+    -- we can assume that commands always have at least one position (see `parseCommand`)
+    let range := (mkNullNode #[stx, endStx]).getRange?.get!.toLspRange text
+    (DocumentSymbol.mk {
+      name
+      kind
+      range
+      selectionRange := selection.getRange? |>.map (·.toLspRange text) |>.getD range
+      children? := syms.toArray
+    } :: syms', stxs'')
 
 def noHighlightKinds : Array SyntaxNodeKind := #[
   -- usually have special highlighting by the client
