src/Std/Data/HashMap.lean
@@ -181,6 +181,9 @@ def insert' (m : HashMap α β) (a : α) (b : β) : HashMap α β × Bool :=
 @[inline] def getOp (self : HashMap α β) (idx : α) : Option β :=
   self.find? idx
 
+instance : GetElem (HashMap α β) α (Option β) fun _ _ => True where
+  getElem m k _ := m.find? k
+
 @[inline] def contains (m : HashMap α β) (a : α) : Bool :=
   match m with
   | ⟨ m, _ ⟩ => m.contains a
